defining gen order

src/NoSync2Stutter.v
@@ -15,6 +15,512 @@ From Fairness Require Export Mod ModSimNoSync ModSimStutter.
 
 Set Implicit Arguments.
 
+Section GENORDER.
+  Context `{M: URA.t}.
+
+  Variable state_src: Type.
+  Variable state_tgt: Type.
+
+  Variable _ident_src: ID.
+  Definition ident_src := sum_tid _ident_src.
+  Variable _ident_tgt: ID.
+  Definition ident_tgt := sum_tid _ident_tgt.
+
+  Variable wf_src: WF.
+  Variable wf_tgt: WF.
+
+  Let srcE := ((@eventE _ident_src +' cE) +' sE state_src).
+  Let tgtE := ((@eventE _ident_tgt +' cE) +' sE state_tgt).
+
+  Variable wf_stt: WF.
+
+  Let shared :=
+    (TIdSet.t *
+       (@imap ident_src wf_src) *
+       (@imap ident_tgt wf_tgt) *
+       state_src *
+       state_tgt *
+       URA.car)%type.
+
+  Let shared_rel: Type := shared -> Prop.
+
+  Variable I: shared_rel.
+
+  Variant __geno
+          (tid: thread_id)
+          (* (geno: forall R_src R_tgt (RR: R_src -> R_tgt -> URA.car -> shared_rel), bool -> bool -> URA.car -> (wf_stt.(T) * itree srcE R_src) -> itree tgtE R_tgt -> shared_rel) *)
+          (_geno: forall R_src R_tgt (RR: R_src -> R_tgt -> URA.car -> shared_rel),bool -> bool -> URA.car -> (wf_stt.(T) * itree srcE R_src) -> itree tgtE R_tgt -> shared_rel)
+          R_src R_tgt (RR: R_src -> R_tgt -> URA.car -> shared_rel)
+    :
+    bool -> bool -> URA.car -> (wf_stt.(T) * itree srcE R_src) -> itree tgtE R_tgt -> shared_rel :=
+  | geno_ret
+      f_src f_tgt r_ctx o o0
+      ths im_src im_tgt st_src st_tgt r_shared
+      r_src r_tgt
+      (LT: wf_stt.(lt) o0 o)
+      (GENO: RR r_src r_tgt r_ctx (ths, im_src, im_tgt, st_src, st_tgt, r_shared))
+    :
+    __geno tid geno _geno RR f_src f_tgt r_ctx (o, Ret r_src) (Ret r_tgt) (ths, im_src, im_tgt, st_src, st_tgt, r_shared)
+
+  | geno_tauL
+      f_src f_tgt r_ctx o
+      ths im_src im_tgt st_src st_tgt r_shared
+      itr_src itr_tgt
+      (GENO: _geno _ _ RR true f_tgt r_ctx (o, itr_src) itr_tgt (ths, im_src, im_tgt, st_src, st_tgt, r_shared))
+    :
+    __geno tid geno _geno RR f_src f_tgt r_ctx (o, Tau itr_src) itr_tgt (ths, im_src, im_tgt, st_src, st_tgt, r_shared)
+  | geno_chooseL
+      f_src f_tgt r_ctx o
+      ths im_src im_tgt st_src st_tgt r_shared
+      X ktr_src itr_tgt
+      (GENO: exists x, _geno _ _ RR true f_tgt r_ctx (o, ktr_src x) itr_tgt (ths, im_src, im_tgt, st_src, st_tgt, r_shared))
+    :
+    __geno tid geno _geno RR f_src f_tgt r_ctx (o, trigger (Choose X) >>= ktr_src) itr_tgt (ths, im_src, im_tgt, st_src, st_tgt, r_shared)
+  | geno_putL
+      f_src f_tgt r_ctx o
+      ths im_src im_tgt st_src st_tgt r_shared
+      st ktr_src itr_tgt
+      (GENO: _geno _ _ RR true f_tgt r_ctx (o, ktr_src tt) itr_tgt (ths, im_src, im_tgt, st, st_tgt, r_shared))
+    :
+    __geno tid geno _geno RR f_src f_tgt r_ctx (o, trigger (Put st) >>= ktr_src) itr_tgt (ths, im_src, im_tgt, st_src, st_tgt, r_shared)
+  | geno_getL
+      f_src f_tgt r_ctx o
+      ths im_src im_tgt st_src st_tgt r_shared
+      ktr_src itr_tgt
+      (GENO: _geno _ _ RR true f_tgt r_ctx (o, ktr_src st_src) itr_tgt (ths, im_src, im_tgt, st_src, st_tgt, r_shared))
+    :
+    __geno tid geno _geno RR f_src f_tgt r_ctx (o, trigger (@Get _) >>= ktr_src) itr_tgt (ths, im_src, im_tgt, st_src, st_tgt, r_shared)
+  | geno_tidL
+      f_src f_tgt r_ctx o
+      ths im_src im_tgt st_src st_tgt r_shared
+      ktr_src itr_tgt
+      (GENO: _geno _ _ RR true f_tgt r_ctx (o, ktr_src tid) itr_tgt (ths, im_src, im_tgt, st_src, st_tgt, r_shared))
+    :
+    __geno tid geno _geno RR f_src f_tgt r_ctx (o, trigger (GetTid) >>= ktr_src) itr_tgt (ths, im_src, im_tgt, st_src, st_tgt, r_shared)
+  | geno_UB
+      f_src f_tgt r_ctx o
+      ths im_src im_tgt st_src st_tgt r_shared
+      ktr_src itr_tgt
+    :
+    __geno tid geno _geno RR f_src f_tgt r_ctx (o, trigger (Undefined) >>= ktr_src) itr_tgt (ths, im_src, im_tgt, st_src, st_tgt, r_shared)
+  | geno_fairL
+      f_src f_tgt r_ctx o
+      ths im_src0 im_tgt st_src st_tgt r_shared
+      f ktr_src itr_tgt
+      (GENO: exists im_src1,
+          (<<FAIR: fair_update im_src0 im_src1 (sum_fmap_r f)>>) /\
+            (<<GENO: _geno _ _ RR true f_tgt r_ctx (o, ktr_src tt) itr_tgt (ths, im_src1, im_tgt, st_src, st_tgt, r_shared)>>))
+    :
+    __geno tid geno _geno RR f_src f_tgt r_ctx (o, trigger (Fair f) >>= ktr_src) itr_tgt (ths, im_src0, im_tgt, st_src, st_tgt, r_shared)
+
+  | geno_tauR
+      f_src f_tgt r_ctx o
+      ths im_src im_tgt st_src st_tgt r_shared
+      itr_src itr_tgt
+      (GENO: _geno _ _ RR f_src true r_ctx (o, itr_src) itr_tgt (ths, im_src, im_tgt, st_src, st_tgt, r_shared))
+    :
+    __geno tid geno _geno RR f_src f_tgt r_ctx (o, itr_src) (Tau itr_tgt) (ths, im_src, im_tgt, st_src, st_tgt, r_shared)
+  | geno_chooseR
+      f_src f_tgt r_ctx o
+      ths im_src im_tgt st_src st_tgt r_shared
+      X itr_src ktr_tgt
+      (GENO: forall x, _geno _ _ RR f_src true r_ctx (o, itr_src) (ktr_tgt x) (ths, im_src, im_tgt, st_src, st_tgt, r_shared))
+    :
+    __geno tid geno _geno RR f_src f_tgt r_ctx (o, itr_src) (trigger (Choose X) >>= ktr_tgt) (ths, im_src, im_tgt, st_src, st_tgt, r_shared)
+  | geno_putR
+      f_src f_tgt r_ctx o
+      ths im_src im_tgt st_src st_tgt r_shared
+      st itr_src ktr_tgt
+      (GENO: _geno _ _ RR f_src true r_ctx (o, itr_src) (ktr_tgt tt) (ths, im_src, im_tgt, st_src, st, r_shared))
+    :
+    __geno tid geno _geno RR f_src f_tgt r_ctx (o, itr_src) (trigger (Put st) >>= ktr_tgt) (ths, im_src, im_tgt, st_src, st_tgt, r_shared)
+  | geno_getR
+      f_src f_tgt r_ctx o
+      ths im_src im_tgt st_src st_tgt r_shared
+      itr_src ktr_tgt
+      (GENO: _geno _ _ RR f_src true r_ctx (o, itr_src) (ktr_tgt st_tgt) (ths, im_src, im_tgt, st_src, st_tgt, r_shared))
+    :
+    __geno tid geno _geno RR f_src f_tgt r_ctx (o, itr_src) (trigger (@Get _) >>= ktr_tgt) (ths, im_src, im_tgt, st_src, st_tgt, r_shared)
+  | geno_tidR
+      f_src f_tgt r_ctx o
+      ths im_src im_tgt st_src st_tgt r_shared
+      itr_src ktr_tgt
+      (GENO: _geno _ _ RR f_src true r_ctx (o, itr_src) (ktr_tgt tid) (ths, im_src, im_tgt, st_src, st_tgt, r_shared))
+    :
+    __geno tid geno _geno RR f_src f_tgt r_ctx (o, itr_src) (trigger (GetTid) >>= ktr_tgt) (ths, im_src, im_tgt, st_src, st_tgt, r_shared)
+  | geno_fairR
+      f_src f_tgt r_ctx o
+      ths im_src im_tgt0 st_src st_tgt r_shared
+      f itr_src ktr_tgt
+      (GENO: forall im_tgt1
+                   (FAIR: fair_update im_tgt0 im_tgt1 (sum_fmap_r f)),
+          (<<GENO: _geno _ _ RR f_src true r_ctx (o, itr_src) (ktr_tgt tt) (ths, im_src, im_tgt1, st_src, st_tgt, r_shared)>>))
+    :
+    __geno tid geno _geno RR f_src f_tgt r_ctx (o, itr_src) (trigger (Fair f) >>= ktr_tgt) (ths, im_src, im_tgt0, st_src, st_tgt, r_shared)
+
+  | geno_observe
+      f_src f_tgt r_ctx o
+      ths im_src im_tgt st_src st_tgt r_shared
+      fn args ktr_src ktr_tgt
+      (GENO: forall ret,
+          _geno _ _ RR true true r_ctx (o, ktr_src ret) (ktr_tgt ret) (ths, im_src, im_tgt, st_src, st_tgt, r_shared))
+    :
+    __geno tid geno _geno RR f_src f_tgt r_ctx (o, trigger (Observe fn args) >>= ktr_src) (trigger (Observe fn args) >>= ktr_tgt) (ths, im_src, im_tgt, st_src, st_tgt, r_shared)
+
+  | geno_yieldR
+      f_src f_tgt r_ctx0 o0
+      ths0 im_src0 im_tgt0 st_src0 st_tgt0 r_shared0
+      r_own r_shared
+      ktr_src ktr_tgt
+      (INV: I (ths0, im_src0, im_tgt0, st_src0, st_tgt0, r_shared))
+      (VALID: URA.wf (r_shared ⋅ r_own ⋅ r_ctx0))
+      (GENO: forall ths1 im_src1 im_tgt1 st_src1 st_tgt1 r_shared1 r_ctx1
+               (INV: I (ths1, im_src1, im_tgt1, st_src1, st_tgt1, r_shared1))
+               (VALID: URA.wf (r_shared1 ⋅ r_own ⋅ r_ctx1))
+               im_tgt2
+               (TGT: fair_update im_tgt1 im_tgt2 (sum_fmap_l (tids_fmap tid ths1))),
+        exists o1,
+            (<<GENO: _geno _ _ RR f_src true r_ctx1 (o1, trigger (Yield) >>= ktr_src) (ktr_tgt tt) (ths1, im_src1, im_tgt2, st_src1, st_tgt1, r_shared1)>>) /\
+              (<<STUTTER: wf_stt.(lt) o1 o0>>))
+    :
+    __geno tid geno _geno RR f_src f_tgt r_ctx0 (o0, trigger (Yield) >>= ktr_src) (trigger (Yield) >>= ktr_tgt) (ths0, im_src0, im_tgt0, st_src0, st_tgt0, r_shared0)
+  | geno_yieldL
+      f_src f_tgt r_ctx o0
+      ths im_src0 im_tgt st_src st_tgt r_shared
+      ktr_src itr_tgt
+      (GENO: exists im_src1 o1,
+          (<<FAIR: fair_update im_src0 im_src1 (sum_fmap_l (tids_fmap tid ths))>>) /\
+            (<<GENO: _geno _ _ RR true f_tgt r_ctx (o1, ktr_src tt) itr_tgt (ths, im_src1, im_tgt, st_src, st_tgt, r_shared)>>))
+    :
+    __geno tid geno _geno RR f_src f_tgt r_ctx (o0, trigger (Yield) >>= ktr_src) itr_tgt (ths, im_src0, im_tgt, st_src, st_tgt, r_shared)
+
+  | geno_progress
+      r_ctx o
+      ths im_src im_tgt st_src st_tgt r_shared
+      itr_src itr_tgt
+      (GENO: ModSimNoSync.lsim I tid RR false false r_ctx itr_src itr_tgt (ths, im_src, im_tgt, st_src, st_tgt, r_shared))
+    :
+    __geno tid geno _geno RR true true r_ctx (o, itr_src) itr_tgt (ths, im_src, im_tgt, st_src, st_tgt, r_shared)
+  .
+
+  Definition lsim (tid: thread_id)
+             R_src R_tgt (RR: R_src -> R_tgt -> URA.car -> shared_rel):
+    bool -> bool -> URA.car -> (wf_stt.(T) * itree srcE R_src) -> itree tgtE R_tgt -> shared_rel :=
+    paco9 (fun r => pind9 (__lsim tid r) top9) bot9 R_src R_tgt RR.
+
+  Lemma __lsim_mon tid:
+    forall r r' (LE: r <9= r'), (__lsim tid r) <10= (__lsim tid r').
+  Proof.
+    ii. inv PR; try (econs; eauto; fail).
+    eapply lsim_yieldR; eauto. i. hexploit LSIM; eauto. i. des. esplits; eauto.
+  Qed.
+
+  Lemma _lsim_mon tid: forall r, monotone9 (__lsim tid r).
+  Proof.
+    ii. inv IN; try (econs; eauto; fail).
+    { des. econs; eauto. }
+    { des. econs; eauto. }
+    { econs. i. eapply LE. eapply LSIM. eauto. }
+    (* { econs; eauto. i. specialize (LSIM _ _ _ _ _ _ _ INV0 VALID0 _ TGT). des. esplits; eauto. } *)
+    { des. econs; esplits; eauto. }
+  Qed.
+
+  Lemma lsim_mon tid: forall q, monotone9 (fun r => pind9 (__lsim tid r) q).
+  Proof.
+    ii. eapply pind9_mon_gen; eauto.
+    ii. eapply __lsim_mon; eauto.
+  Qed.
+
+  Variant lsim_resetC
+          (r: forall R_src R_tgt (RR: R_src -> R_tgt -> URA.car -> shared_rel), bool -> bool -> URA.car -> (wf_stt.(T) * itree srcE R_src) -> itree tgtE R_tgt -> shared_rel)
+          R_src R_tgt (RR: R_src -> R_tgt -> URA.car -> shared_rel)
+    :
+    bool -> bool -> URA.car -> (wf_stt.(T) * itree srcE R_src) -> itree tgtE R_tgt -> shared_rel :=
+    | lsim_resetC_intro
+        src tgt shr r_ctx
+        ps0 pt0 ps1 pt1
+        (REL: r _ _ RR ps1 pt1 r_ctx src tgt shr)
+        (SRC: ps1 = true -> ps0 = true)
+        (TGT: pt1 = true -> pt0 = true)
+      :
+      lsim_resetC r RR ps0 pt0 r_ctx src tgt shr
+  .
+
+  Lemma lsim_resetC_spec tid
+    :
+    lsim_resetC <10= gupaco9 (fun r => pind9 (__lsim tid r) top9) (cpn9 (fun r => pind9 (__lsim tid r) top9)).
+  Proof.
+    eapply wrespect9_uclo; eauto with paco.
+    { eapply lsim_mon. }
+    econs.
+    { ii. inv IN. econs; eauto. }
+    i. inv PR. eapply GF in REL.
+    eapply pind9_acc in REL.
+    instantiate (1:= (fun R0 R1 (RR: R0 -> R1 -> URA.car -> shared_rel) ps1 pt1 r_ctx src tgt shr =>
+                        forall ps0 pt0,
+                          (ps1 = true -> ps0 = true) ->
+                          (pt1 = true -> pt0 = true) ->
+                          pind9 (__lsim tid (rclo9 lsim_resetC r)) top9 R0 R1 RR ps0 pt0 r_ctx src tgt shr)) in REL; eauto.
+    ss. i. eapply pind9_unfold in PR.
+    2:{ eapply _lsim_mon. }
+    rename PR into LSIM. inv LSIM.
+
+    { eapply pind9_fold. econs; eauto. }
+
+    { destruct LSIM0 as [LSIM0 IND]. clear LSIM0.
+      eapply pind9_fold. eapply lsim_tauL. split; ss.
+      hexploit IH; eauto.
+    }
+
+    { des. eapply pind9_fold. eapply lsim_chooseL. esplits; eauto. split; ss.
+      destruct LSIM0 as [LSIM0 IND]. hexploit IH; eauto.
+    }
+
+    { eapply pind9_fold. eapply lsim_putL. split; ss.
+      destruct LSIM0 as [LSIM0 IND]. hexploit IH; eauto.
+    }
+
+    { eapply pind9_fold. eapply lsim_getL. split; ss.
+      destruct LSIM0 as [LSIM0 IND]. hexploit IH; eauto.
+    }
+
+    { eapply pind9_fold. eapply lsim_tidL. split; ss.
+      destruct LSIM0 as [LSIM0 IND]. hexploit IH; eauto.
+    }
+
+    { eapply pind9_fold. eapply lsim_UB. }
+
+    { des. eapply pind9_fold. eapply lsim_fairL. esplits; eauto. split; ss.
+      destruct LSIM as [LSIM IND]. hexploit IH; eauto.
+    }
+
+    { destruct LSIM0 as [LSIM0 IND]. clear LSIM0.
+      eapply pind9_fold. eapply lsim_tauR. split; ss.
+      hexploit IH. eauto. all: eauto.
+    }
+
+    { eapply pind9_fold. eapply lsim_chooseR. i. split; ss. specialize (LSIM0 x).
+      destruct LSIM0 as [LSIM0 IND]. hexploit IH; eauto.
+    }
+
+    { eapply pind9_fold. eapply lsim_putR. split; ss.
+      destruct LSIM0 as [LSIM0 IND]. hexploit IH; eauto.
+    }
+
+    { eapply pind9_fold. eapply lsim_getR. split; ss.
+      destruct LSIM0 as [LSIM0 IND]. hexploit IH; eauto.
+    }
+
+    { eapply pind9_fold. eapply lsim_tidR. split; ss.
+      destruct LSIM0 as [LSIM0 IND]. hexploit IH; eauto.
+    }
+
+    { eapply pind9_fold. eapply lsim_fairR. i. split; ss. specialize (LSIM0 _ FAIR).
+      des. destruct LSIM0 as [LSIM0 IND]. hexploit IH; eauto.
+    }
+
+    { eapply pind9_fold. eapply lsim_observe. i. eapply rclo9_base. auto. }
+
+    { eapply pind9_fold. eapply lsim_yieldR; eauto. i.
+      hexploit LSIM0; eauto. clear LSIM0. intros LSIM0. des. esplits; eauto.
+      eapply rclo9_base. auto.
+    }
+
+    { des. eapply pind9_fold. eapply lsim_yieldL. esplits; eauto. split; ss.
+      destruct LSIM as [LSIM IND]. hexploit IH; eauto.
+    }
+
+    { hexploit H; ss; i. hexploit H0; ss; i. clarify.
+      eapply pind9_fold. eapply lsim_progress. eapply rclo9_base; auto. }
+  Qed.
+
+  Lemma lsim_reset_prog
+        tid
+        R0 R1 (RR: R0 -> R1 -> URA.car -> shared_rel)
+        src tgt shr
+        ps0 pt0 ps1 pt1 r_ctx
+        (LSIM: lsim tid RR ps1 pt1 r_ctx src tgt shr)
+        (SRC: ps1 = true -> ps0 = true)
+        (TGT: pt1 = true -> pt0 = true)
+    :
+    lsim tid RR ps0 pt0 r_ctx src tgt shr.
+  Proof.
+    ginit.
+    { eapply lsim_mon. }
+    { eapply cpn9_wcompat. eapply lsim_mon. }
+    guclo lsim_resetC_spec.
+    { eapply lsim_mon. }
+    econs; eauto. gfinal.
+    { eapply lsim_mon. }
+    right. auto.
+  Qed.
+
+  Lemma lsim_set_prog
+        tid
+        R0 R1 (RR: R0 -> R1 -> URA.car -> shared_rel)
+        r_ctx src tgt shr
+        (LSIM: lsim tid RR true true r_ctx src tgt shr)
+    :
+    forall ps pt, lsim tid RR ps pt r_ctx src tgt shr.
+  Proof.
+    i. revert_until tid. pcofix CIH. i.
+    remember true as ps0 in LSIM at 1. remember true as pt0 in LSIM at 1.
+    move LSIM before CIH. revert_until LSIM. punfold LSIM.
+    2:{ eapply lsim_mon. }
+    eapply pind9_acc in LSIM.
+
+    { instantiate (1:= (fun R0 R1 (RR: R0 -> R1 -> URA.car -> shared_rel) ps0 pt0 r_ctx src tgt shr =>
+                          ps0 = true ->
+                          pt0 = true ->
+                          forall ps pt,
+                            paco9
+                              (fun r0 =>
+                                 pind9 (__lsim tid r0) top9) r R0 R1 RR ps pt r_ctx src tgt shr)) in LSIM; auto. }
+
+    ss. clear ps0 pt0 r_ctx src tgt shr LSIM.
+    intros rr DEC IH R0' R1' RR' gps gpt r_ctx src tgt shr LSIM. clear DEC.
+    intros Egps Egpt ps pt.
+    eapply pind9_unfold in LSIM.
+    2:{ eapply _lsim_mon. }
+    inv LSIM.
+
+    { pfold. eapply pind9_fold. econs; eauto. }
+
+    { destruct LSIM0 as [LSIM0 IND]. clear LSIM0.
+      pfold. eapply pind9_fold. eapply lsim_tauL. split; ss.
+      hexploit IH. eauto. all: eauto. i. punfold H. eapply lsim_mon.
+    }
+
+    { des. pfold. eapply pind9_fold. eapply lsim_chooseL. esplits; eauto. split; ss.
+      destruct LSIM0 as [LSIM0 IND]. hexploit IH; eauto. i. punfold H. eapply lsim_mon.
+    }
+
+    { pfold. eapply pind9_fold. eapply lsim_putL. split; ss.
+      destruct LSIM0 as [LSIM0 IND]. hexploit IH; eauto. i. punfold H. eapply lsim_mon.
+    }
+
+    { pfold. eapply pind9_fold. eapply lsim_getL. split; ss.
+      destruct LSIM0 as [LSIM0 IND]. hexploit IH; eauto. i. punfold H. eapply lsim_mon.
+    }
+
+    { pfold. eapply pind9_fold. eapply lsim_tidL. split; ss.
+      destruct LSIM0 as [LSIM0 IND]. hexploit IH; eauto. i. punfold H. eapply lsim_mon.
+    }
+
+    { pfold. eapply pind9_fold. eapply lsim_UB. }
+
+    { des. pfold. eapply pind9_fold. eapply lsim_fairL. esplits; eauto. split; ss.
+      destruct LSIM as [LSIM IND]. hexploit IH; eauto. i. punfold H. eapply lsim_mon.
+    }
+
+    { destruct LSIM0 as [LSIM0 IND]. clear LSIM0.
+      pfold. eapply pind9_fold. eapply lsim_tauR. split; ss.
+      hexploit IH. eauto. all: eauto. i. punfold H. eapply lsim_mon.
+    }
+
+    { pfold. eapply pind9_fold. eapply lsim_chooseR. i. split; ss. specialize (LSIM0 x).
+      destruct LSIM0 as [LSIM0 IND]. hexploit IH; eauto. i. punfold H. eapply lsim_mon.
+    }
+
+    { pfold. eapply pind9_fold. eapply lsim_putR. split; ss.
+      destruct LSIM0 as [LSIM0 IND]. hexploit IH; eauto. i. punfold H. eapply lsim_mon.
+    }
+
+    { pfold. eapply pind9_fold. eapply lsim_getR. split; ss.
+      destruct LSIM0 as [LSIM0 IND]. hexploit IH; eauto. i. punfold H. eapply lsim_mon.
+    }
+
+    { pfold. eapply pind9_fold. eapply lsim_tidR. split; ss.
+      destruct LSIM0 as [LSIM0 IND]. hexploit IH; eauto. i. punfold H. eapply lsim_mon.
+    }
+
+    { pfold. eapply pind9_fold. eapply lsim_fairR. i. split; ss. specialize (LSIM0 _ FAIR).
+      des. destruct LSIM0 as [LSIM0 IND]. hexploit IH; eauto. i. punfold H. eapply lsim_mon.
+    }
+
+    { pfold. eapply pind9_fold. eapply lsim_observe. i. eapply upaco9_mon_bot; eauto. }
+
+    { pfold. eapply pind9_fold. eapply lsim_yieldR; eauto. i.
+      hexploit LSIM0; eauto. clear LSIM0. intros LSIM0. des. esplits; eauto.
+      eapply upaco9_mon_bot; eauto.
+    }
+
+    { des. pfold. eapply pind9_fold. eapply lsim_yieldL. esplits; eauto. split; ss.
+      destruct LSIM as [LSIM IND]. hexploit IH; eauto. i. punfold H. eapply lsim_mon.
+    }
+
+    { pclearbot. eapply paco9_mon_bot. eapply lsim_reset_prog. eauto. all: ss. }
+
+  Qed.
+
+  Definition local_RR {R0 R1} (RR: R0 -> R1 -> Prop) tid:
+    R0 -> R1 -> URA.car -> shared_rel :=
+    fun (r_src: R0) (r_tgt: R1) (r_ctx: URA.car) '(ths2, im_src1, im_tgt1, st_src1, st_tgt1, r_shared1) =>
+      (exists ths3 r_own r_shared2,
+          (<<THS: NatMap.remove tid ths2 = ths3>>) /\
+            (<<VALID: URA.wf (r_shared2 ⋅ r_own ⋅ r_ctx)>>) /\
+            (<<INV: I (ths3, im_src1, im_tgt1, st_src1, st_tgt1, r_shared2)>>) /\
+            (<<RET: RR r_src r_tgt>>)).
+
+  (* Definition local_RR {R0 R1} (RR: R0 -> R1 -> Prop) tid: *)
+  (*   R0 -> R1 -> URA.car -> wf_stt.(T) -> shared_rel := *)
+  (*   fun (r_src: R0) (r_tgt: R1) (r_ctx: URA.car) (o: wf_stt.(T)) '(ths2, im_src1, im_tgt1, st_src1, st_tgt1, r_shared1) => *)
+  (*     (exists ths3 r_own o0 r_shared2, *)
+  (*         (<<THS: NatMap.remove tid ths2 = ths3>>) /\ *)
+  (*           (<<VALID: URA.wf (r_shared2 ⋅ r_own ⋅ r_ctx)>>) /\ *)
+  (*           (<<INV: I (ths3, im_src1, im_tgt1, st_src1, st_tgt1, r_shared2)>>) /\ *)
+  (*           (<<STT: wf_stt.(lt) o0 o>>) /\ *)
+  (*           (<<RET: RR r_src r_tgt>>)). *)
+
+  (* Definition embed_lrr {R0 R1} (LRR: R0 -> R1 -> URA.car -> shared_rel): *)
+  (*   R0 -> R1 -> URA.car -> wf_stt.(T) -> shared_rel := *)
+  (*   fun (r_src: R0) (r_tgt: R1) (r_ctx: URA.car) (o: wf_stt.(T)) shr => *)
+  (*     (<<LSIM: LRR r_src r_tgt r_ctx shr>>) /\ (<<STT: exists o0, wf_stt.(lt) o0 o>>). *)
+
+  Definition local_sim {R0 R1} (RR: R0 -> R1 -> Prop) src tgt :=
+    forall ths0 im_src0 im_tgt0 st_src0 st_tgt0 r_shared0 r_ctx0
+      (INV: I (ths0, im_src0, im_tgt0, st_src0, st_tgt0, r_shared0))
+      tid ths1
+      (THS: TIdSet.add_new tid ths0 ths1)
+      (VALID: URA.wf (r_shared0 ⋅ r_ctx0)),
+    exists r_shared1 r_own,
+      (<<INV: I (ths1, im_src0, im_tgt0, st_src0, st_tgt0, r_shared1)>>) /\
+        (<<VALID: URA.wf (r_shared1 ⋅ r_own ⋅ r_ctx0)>>) /\
+        (forall ths im_src1 im_tgt1 st_src st_tgt r_shared2 r_ctx2
+           (INV: I (ths, im_src1, im_tgt1, st_src, st_tgt, r_shared2))
+           (VALID: URA.wf (r_shared2 ⋅ r_own ⋅ r_ctx2))
+           im_tgt2
+           (TGT: fair_update im_tgt1 im_tgt2 (sum_fmap_l (tids_fmap tid ths))),
+          exists o,
+          exists im_src2, (<<SRC: fair_update im_src1 im_src2 (sum_fmap_l (tids_fmap tid ths))>>) /\
+                       (<<LSIM: forall fs ft,
+                           lsim
+                             tid
+                             (@local_RR R0 R1 RR tid)
+                             fs ft
+                             r_ctx2
+                             (o, src) tgt
+                             (ths, im_src2, im_tgt2, st_src, st_tgt, r_shared2)
+                             >>)).
+
+  (* Definition shared_rel_wf: Prop := *)
+  (*   forall ths im_src0 im_tgt0 st_src st_tgt r_shared0 r_ctx *)
+  (*          (INV: I (ths, im_src0, im_tgt0, st_src, st_tgt, r_shared0)) *)
+  (*          (VALID: URA.wf (r_shared0 ⋅ r_ctx)), *)
+  (*   forall im_tgt1 *)
+  (*          (TGT: fair_update im_tgt0 im_tgt1 (sum_fmap_l (tids_fmap_all ths))), *)
+  (*   exists im_src1 r_shared1, *)
+  (*     (<<SRC: fair_update im_src0 im_src1 (sum_fmap_l (tids_fmap_all ths))>>) /\ *)
+  (*       (<<INV: I (ths, im_src1, im_tgt1, st_src, st_tgt, r_shared1)>>) /\ *)
+  (*       (<<VALID: URA.wf (r_shared1 ⋅ r_ctx)>>). *)
+
+End PRIMIVIESIM.
+#[export] Hint Constructors __lsim: core.
+#[export] Hint Unfold lsim: core.
+#[export] Hint Resolve __lsim_mon: paco.
+#[export] Hint Resolve _lsim_mon: paco.
+#[export] Hint Resolve lsim_mon: paco.
+
 Section PROOF.
 
   Context `{M: URA.t}.
